

# Introduction to Artificial Intelligence

## Homework 3 Resolution by Dino Meng [SM3201466]

---

### Q1. Searching with Heuristics

**A1.**  $C = h^*(S)$ , by direct calculations we can estimate  $h'(X)$  as

$$h'(X) = \frac{1}{2}h(X) \leq \frac{1}{2}h^*(X) \leq h^*(X)$$

Meaning that  $h'$  is admissible thus gives an optimal solution

**A2.**  $C = h^*(S)$ , since that we can similarly estimate  $h'(X)$  as before:

$$h'(X) = \frac{h(X) + h^*(X)}{2} \leq \frac{2h^*(X)}{2} = h^*(X)$$

Proving again that  $h'$  is admissible.

**A3.**  $C \geq h^*(S)$ , as  $h'(X)$  is not admissible. By estimating  $h'$  again, we get the bounds

$$h'(X) \leq h(X) + h^*(X) \leq 2h^*(X)$$

Meaning that in certain cases it could be that  $2h'(X) \geq h'(X) > h'(X)$ , which does not guarantee admissibility for the heuristic.

**A4.**  $C \geq h^*(S)$ , as  $h'$  is admissible. To prove that it is admissible, we first can observe that that  $h'(X) - h(X) \leq 0$  for any node; the idea is that  $h'$  will be lower than  $h$  as it tries to find a node of a lower cost in its “network” of neighbouring nodes. We will prove it by induction on  $h'$ . - Base case: We assume that  $K(X)$  empty, then  $h'(X) \leq h(X)$  which is  $h'(X) - h(X) \leq 0$  - Inductive Case: Assume that for each  $Y \in K(X) \neq \emptyset$  we have that  $h'(Y) - h(Y) \leq 0$ . Then calculating  $h'(X) - h(X)$  we have that

$$h'(X) - h(X) \leq \min_{y \in K(X)} h'(Y) - h(Y) \leq 0$$

Then by making few direct calculations on  $h$ , we can see that:

$$h'(X) \leq \begin{cases} \overbrace{\min_{Y \in K(X)} h'(Y) - h(Y)}^{\leq 0} + h(X), & K(X) \neq \emptyset \\ h(X), & K(X) = \emptyset \end{cases} \leq h(X) \leq h^*(X)$$

proving that  $h'$  is admissible, concluding.

**A5.**  $C \geq h^*(S)$ , as  $h'$  is admissible. Notice that  $\text{cost}(x, y) = h^*(x) - h^*(y)$ . Then the heuristic  $h'$  can be estimated as follows:

$$h'(x) = \begin{cases} \min_{Y \in K(X)} (h(Y) + \text{cost}(X, Y)), & K(X) \neq \emptyset \\ h(X), & K(X) = \emptyset \end{cases} \tag{1}$$

$$\leq \begin{cases} \min_{Y \in K(X)} (h^*(Y) + h^*(X) - h^*(Y)), & K(X) \neq \emptyset \\ h^*(X), & K(X) = \emptyset \end{cases} \tag{2}$$

$$= \begin{cases} h^*(X), & K(X) \neq \emptyset \\ h^*(X), & K(X) = \emptyset \end{cases} = h^*(X) \tag{3}$$

Proving that  $h'$  is admissible, concluding.

**A6.**  $C \geq h^*(S)$ , as  $h'$  is admissible. By the properties of the minimum,

$$\min_{Y \in K(X) + \{X\}} h(Y) \leq h(X)$$

So then

$$h'(X) \leq h(X) \leq h^*(X)$$

proving  $h'$  is admissible.

**ii.** The only heuristic which is surely to dominate  $h$  is the second one, as we are taking the average between  $h$  and  $h^*$  so since that  $h^* \geq h$  surely so will the average dominate  $h$ . The rest are either not admissible or are proven to be dominated by  $h$ .

**B1.**  $h'$  is consistent, to verify it we can make direct calculations and using the fact that  $h$  is consistent:

$$h'(X) = \frac{1}{2}h(X) \tag{4}$$

$$\leq \frac{1}{2}(c(X, Y) + h(Y)) \tag{5}$$

$$= \frac{1}{2}c(X, Y) + \frac{1}{2}h(Y) \tag{6}$$

$$= \frac{1}{2}c(X, Y) + h'(Y) \tag{7}$$

$$\leq c(X, Y) + h'(Y) \tag{8}$$

Which is the definition of consistency on  $h'$ , concluding.

**B2.** Similarly to B1,  $h'$  is consistent and we can verify it with direct calculations:

$$h'(X) = \frac{h(X) + h^*(X)}{2} \tag{9}$$

$$\leq \frac{c(X, Y) + h(Y) + h^*(X)}{2} \tag{10}$$

$$= \frac{h^*(X) - h^*(Y) + h(Y) + h^*(X) + h^*(Y) - h^*(Y)}{2} \tag{11}$$

$$= \frac{2c(X, Y)}{2} + h'(Y) \tag{12}$$

$$= c(X, Y) + h'(Y) \tag{13}$$

Concluding.

**B3.**  $C \geq h^*(S)$ : If  $h'$  is not admissible, then it cannot be consistent (as consistency implies admissibility).

**B4.**  $C = h^*(S)$ : we can see that  $h'$  is consistent. To prove it, we can see that by the properties of the minimum that

$$\forall Y \in K(X), h(X) \leq h'(Y) - h(Y) + h(X)$$

which implies

$$h'(Y) \leq h(X) - h(Y) + c(X, Y)$$

So

$$h'(Y) \leq c(X, Y) + h(X)$$

Which implies  $h'$  is consistent, concluding.

**B5.**  $C = h^*(S)$ : we can see that  $h'$  is consistent. Before proving its consistency, let us observe that if  $h$  is consistent then  $h' \geq h$ : in fact we have that

$$h(X) - h(Y) \leq c(X, Y) \iff h(X) \leq c(X, Y) + h(Y)$$

Then applying it for  $Y = \min\{Y \in K(X) : h(Y) + c(X, Y)\}$ , we have that

$$h(X) \leq h'(X)$$

Now let us prove the consistency. By definition, if we have that  $K(X) \neq 0$  then

$$h'(X) \leq h(Y) + c(X, Y), \forall Y \in K(X)$$

For dominance we have that

$$h'(X) \leq h'(Y) + c(X, Y)$$

concluding the proof.

**B6.** We cannot be sure that it is consistent, in fact we have a counterexample for the graph  $G = \{S, A, B, G\}$  with weights  $SA = 4, AB = 2, SB = 8, BG = 42$ .

**ii.**  $h'$  is consistent and dominant over  $h$  for **B2** and **B5**.

**C1.** Bob's conclusion is wrong, because  $h''$  can be inadmissible for  $X_0 = G$  as it becomes negative for  $h''(X_0)$ .

---

## Q2. Iterative Deepening Search

a)

- i)  $+\infty$
- ii) False
- iii) new\_limit
- iv) cutoff
- v)  $\min(\text{new\_limit}, f[\text{child\_node}])$
- vi) True
- vii) new\_limit

**b)** The number of times that iterative deepening  $A^*$  expands a node is greater than or equal the number of times  $A^*$  will expand a node, because the variant runs the original algorithms more times for each different limit value, so it tends to re-explore certain nodes